src/bijection.v
@@ -8,47 +8,194 @@ Require stream.
 Require encode.
 Require decode.
 
+Ltac mcase e H p HR :=
+  case_eq e; try intros p HR; try intros HR; rewrite HR in H;
+  try destruct p; try discriminate.
+
 Fact positive_size_lt0: forall (p: positive), Pos.size_nat p > 0.
 Proof.
   induction p; simpl; omega.
 Qed.
 
-Definition bijection {A}
-           (dec: stream.bit -> option (A * stream.bit))
-           (enc: A -> stream.bit -> stream.bit)
-           (a: A) :=
-  forall (a: A)(s s': stream.bit),
-    (dec s') = Some (a, s) <-> (enc a s) = s'.
-
-Lemma number: forall (bits: nat) (n: N),
-    (N.size_nat n) <= (S bits) ->
-    bijection (decode.number (S bits)) (encode.number (S bits)) n.
+Lemma number_encdec:
+  forall (bits: nat) (n: N) (s: stream.bit),
+    (N.size_nat n) <= bits ->
+    decode.number bits (encode.number bits n s) = Some (n, s).
 Proof.
-  unfold bijection, decode.number, decode.number_rec.
-  induction bits; split; intros; destruct s; simpl.
-  - destruct n; try destruct p; try trivial;
-      try (contradict H; simpl; apply gt_not_le;
-           specialize positive_size_lt0 with (p);
-           omega).
-    + case_eq (stream.take s'); intros; rewrite H1 in H0.
-      * destruct p. simpl in H0. admit.
-      * admit.
-    + admit.
+  induction bits; intros; simpl.
+  - destruct n.
+    + reflexivity.
+    + contradict H. simpl.
+      apply gt_not_le. apply positive_size_lt0.
   - admit.
 Admitted.
 
-Lemma condition: forall (c: ast.condition),
-    bijection decode.condition encode.condition c.
+Lemma number_decenc:
+  forall (bits: nat) (n: N) (s s': stream.bit),
+    decode.number bits s = Some (n, s') ->
+    encode.number bits n s' = s.
+Proof.
+  induction bits; intros; simpl; simpl in H.
+  - injection H. intros. symmetry. assumption.
+  - mcase (stream.take s) H p H0.
+    mcase (decode.number bits t) H p H1.
+    admit.
+Admitted.
+
+Ltac number_encdec := rewrite number_encdec; try (simpl; omega).
+
+Fact decode_expect:
+  forall (bits: nat) (e: N) (s s': stream.bit),
+    decode.expect bits e s = Some (tt, s') <->
+    decode.number bits s = Some (e, s').
+Proof.
+  unfold decode.expect.
+  split; intros.
+  - mcase (decode.number bits s) H p H0.
+    mcase (n =? e)%N H p H1.
+    injection H. intros. subst.
+    apply Neqb_ok in H1. rewrite H1.
+    reflexivity.
+  - rewrite H. rewrite N.eqb_refl.
+    reflexivity.
+Qed.
+
+Ltac expect_encdec :=
+  unfold decode.expect; number_encdec; rewrite N.eqb_refl.
+
+Ltac plain_number_encdec :=
+  intros;
+  rewrite number_encdec;
+  try reflexivity;
+  try assumption.
+
+Fact register_encdec: forall (n: N) (s: stream.bit),
+    (N.size_nat n) <= ast.register_bits ->
+    decode.register (encode.register (ast.reg n) s)
+    = Some (ast.reg n, s).
+Proof.
+  unfold encode.register, decode.register.
+  plain_number_encdec.
+Qed.
+
+Fact immediate_encdec: forall (n: N) (s: stream.bit),
+    (N.size_nat n) <= ast.constant_bits ->
+    decode.immediate (encode.immediate (ast.imm n) s)
+    = Some (ast.imm n, s).
+Proof.
+  unfold encode.immediate, decode.immediate.
+  plain_number_encdec.
+Qed.
+
+Fact displacement_encdec: forall (n: N) (s: stream.bit),
+    (N.size_nat n) <= ast.constant_bits ->
+    decode.displacement (encode.displacement (ast.dsp n) s)
+    = Some (ast.dsp n, s).
+Proof.
+  unfold encode.displacement, decode.displacement.
+  plain_number_encdec.
+Qed.
+
+Fact destination_encdec: forall (n: N) (s: stream.bit),
+    (N.size_nat n) <= ast.constant_bits ->
+    decode.destination (encode.destination (ast.dst n) s)
+    = Some (ast.dst n, s).
+Proof.
+  unfold encode.destination, decode.destination.
+  plain_number_encdec.
+Qed.
+
+Fact condition_encdec: forall (c: ast.condition) (s: stream.bit),
+    decode.condition (encode.condition c s) = Some (c, s).
 Proof.
 Admitted.
 
-Theorem instruction: forall (i: ast.instruction),
-    bijection decode.instruction encode.instruction i.
+Fact operator_encdec: forall (op: ast.operator) (s: stream.bit),
+    decode.operator (encode.operator op s) = Some (op, s).
 Proof.
 Admitted.
 
-Lemma instructions: forall (ins: ast.instructions) (s: stream.bit),
-    (decode.instructions s) = Some ins
-    <-> (encode.instructions ins stream.empty) = s.
+Fact register_decenc: forall (n: N) (s s': stream.bit),
+    decode.register s = Some (ast.reg n, s') ->
+    encode.register (ast.reg n) s' = s.
 Proof.
+  unfold encode.register, decode.register.
+  intros.
+  apply number_decenc.
+  mcase (decode.number ast.register_bits s) H p H0.
+  injection H. intros. subst. reflexivity.
+Qed.
+
+Ltac register_encdec r := destruct r; rewrite register_encdec.
+Ltac immediate_encdec i := destruct i; rewrite immediate_encdec.
+Ltac displacement_encdec i := destruct i; rewrite displacement_encdec.
+Ltac destination_encdec i := destruct i; rewrite destination_encdec.
+
+Lemma instruction_encdec:
+  forall (i: ast.instruction) (s: stream.bit),
+    decode.instruction (encode.instruction i s) = Some (i, s).
+Proof.
+  unfold decode.instruction, encode.instruction.
+  intros.
+  destruct i; rewrite number_encdec; try (simpl; omega).
+  - expect_encdec. reflexivity.
+  - expect_encdec. reflexivity.
+  - unfold decode.rrmovl.
+    rewrite condition_encdec.
+    register_encdec r.
+    register_encdec r0.
+    reflexivity.
+    admit. admit. (* TODO: limit values *)
+  - unfold decode.irmovl.
+    expect_encdec.
+    expect_encdec.
+    register_encdec r.
+    immediate_encdec i.
+    reflexivity.
+    admit. admit. (* TODO: limit values *)
+  - unfold decode.rmmovl.
+    expect_encdec.
+    register_encdec r.
+    register_encdec r0.
+    displacement_encdec d.
+    reflexivity.
+    admit. admit. admit. (* TODO: limit values *)
+  - unfold decode.mrmovl.
+    expect_encdec.
+    register_encdec r.
+    register_encdec r0.
+    displacement_encdec d.
+    reflexivity.
+    admit. admit. admit. (* TODO: limit values *)
+  - unfold decode.OPl.
+    rewrite operator_encdec.
+    register_encdec r.
+    register_encdec r0.
+    reflexivity.
+    admit. admit. (* TODO: limit values *)
+  - unfold decode.jump.
+    rewrite condition_encdec.
+    destination_encdec d.
+    reflexivity.
+    admit. (* TODO: limit values *)
+  - unfold decode.call.
+    expect_encdec.
+    destination_encdec d.
+    reflexivity.
+    admit. (* TODO: limit values *)
+  - unfold decode.ret.
+    expect_encdec.
+    reflexivity.
+  - unfold decode.pushl.
+    expect_encdec.
+    register_encdec r.
+    expect_encdec.
+    reflexivity.
+    admit. (* TODO: limit values *)
+  - unfold decode.popl.
+    expect_encdec.
+    register_encdec r.
+    expect_encdec.
+    reflexivity.
+    admit. (* TODO: limit values *)
 Admitted.
